Reworked has_skew_product for lists.

utilities/LimitMonads.v
@@ -34,16 +34,30 @@ Section LimitMonads.
 Definition lcons {X : Type} : prod (list X) X -> list X :=
   fun xl_x => cons (snd xl_x) (fst xl_x).
 
-Definition is_infinite_skew_product {M : Type -> Type} {_ : Monad M} {X : Type}
+Definition is_list_infinite_skew_product {M : Type -> Type} {_ : Monad M} {X : Type}
   (F : (list X) -> M X) (Finf : M (nat -> X)) :=
     (Mlift (proj 0) Finf = Mpure nil) /\
       forall (n:nat),
         Mlift lcons (Mright_skew (Mlift (proj n) Finf) F) =
         Mlift (proj (S n)) Finf.
 
-Definition has_infinite_skew_product (M : Type -> Type) (_ : Monad M) :=
+Definition exists_list_infinite_skew_product (M : Type -> Type) (_ : Monad M) :=
   forall (X : Type) (F : (list X) -> M X),
     exists (Finf : M (nat -> X)),
-      is_infinite_skew_product F Finf.
+      is_list_infinite_skew_product F Finf.
+
+Definition has_list_infinite_skew_product (M : Type -> Type) (_ : Monad M) :=
+  forall (X : Type) (F : (list X) -> M X),
+    sig (fun Finf : M (nat -> X) => is_list_infinite_skew_product F Finf).
+
+Definition list_infinite_skew_product (M : Type -> Type) (Monad_M : Monad M) (H : has_list_infinite_skew_product  M Monad_M)
+  {X : Type} (F : (list X) -> M X) : M (nat -> X).
+Proof.
+  unfold has_list_infinite_skew_product in H.
+  specialize (H X F).
+  destruct H as [Finf _].
+  exact Finf.
+Qed.
+
 
 End LimitMonads.
